theories/paris/examples/security_definitions.v
@@ -1,0 +1,86 @@
+From clutch Require Import lib.flip.
+From clutch.paris Require Import paris map list.
+Set Default Proof Using "Type*".
+
+
+Section bounded_oracle.
+  Local Opaque INR.
+
+  (** Bounded Oracles *)
+  Definition q_calls (MAX : Z) : val :=
+    λ:"Q" "f" "g",
+      let: "counter" := ref #0 in
+      λ:"x", if: (BinOp AndOp (! "counter" < "Q") (BinOp AndOp (#0 ≤ "x") ("x" < #MAX)))
+             then ("counter" <- !"counter" + #1 ;; "f" "x")
+             else "g" "x".
+End bounded_oracle.
+
+
+Section symmetric.
+
+  (** A symmetric encryption [scheme] is given by three functions (keygen, encrypt, decrypt).
+
+The set of keys, messages, and ciphertexts are modelled by finite sets of integers [0, Key], [0, Input], and [0, Output].
+   *)
+
+  Variable Key Message Cipher : nat.
+
+  Let keygen scheme : expr := Fst scheme.
+  Let enc scheme : expr := Fst (Snd scheme).
+  Let rand_cipher scheme : expr := Snd (Snd scheme).
+
+  Section CPA.
+
+    (** Indistinguishability of Chosen Plaintext Attacks security
+      for symmetric/private key encryption.
+
+Real vs random variant (sometimes called "CPA$").
+
+References:
+- Definition 7.2, Mike Rosulek, 2020, The Joy of Cryptography.
+- Definition 3.22, Jonathan Katz and Yehuda Lindell, 2021, Introduction to Modern Cryptography (3rd edition).
+
+Our definition deviates from Rosulek's and Katz/Lindell in that we wrap the encryption oracle with [q_calls] to enforce the bound [Q] on the number of oracle calls, while loc. cit. rely on the assumption that the adversary runs in polynomial time in the security parameter.
+
+Our definition further differs from Katz/Lindell in that, depending on the value of [b], the encryption oracle either encrypts the adversary's message or return a random ciphertext, whereas in Katz/Lindell, the encryption oracle encrypts one of two messages provided by the adversary. These two notions are equivalent by Claim 7.3 in Rosulek's book.
+     *)
+
+
+    Let q_calls := q_calls Message.
+    Definition CPA : val :=
+      λ:"b" "adv" "scheme" "Q",
+        let: "rr_key_b" :=
+          let: "key" := keygen "scheme" #() in
+          (* let: "enc_key" := enc "scheme" "key" in *)
+          if: "b" then
+            (* "enc_key" *)
+            enc "scheme" "key"
+          else
+            rand_cipher "scheme" in
+        let: "oracle" := q_calls "Q" "rr_key_b" (rand_cipher "scheme") in
+        let: "b'" := "adv" "oracle" in
+        "b'".
+
+  End CPA.
+
+End symmetric.
+
+Section PRF.
+
+  Variable Key Input Output : nat.
+
+  (* An idealised random function family. *)
+  Definition random_function : val :=
+    λ: "_key",
+      (* Create a reference to a functional map *)
+      let: "mapref" := init_map #() in
+      λ: "x",
+        match: get "mapref" "x" with
+        | SOME "y" => "y"
+        | NONE =>
+            let: "y" := (rand #Output) in
+            set "mapref" "x" "y";;
+            "y"
+        end.
+
+End PRF.
